nondeterministic_dataflow/table_1/B2.thy
@@ -10,38 +10,38 @@ section \<open>Axiom B2: Neutral element of parallel composition\<close>
 lemma B2_1:
   \<open>(op \<parallel> (\<I> :: (0, 0, 'd) op)) ~ map_op Inl Inl op\<close>
   unfolding pcomp_op_def
-proof (coinduction arbitrary: op rule: bisim_coinduct_upto'')
+proof (coinduction arbitrary: op rule: bisim_coinduct)
   case SIM1
   then show ?case 
     apply -
     explore (auto elim!: step_comp_op_elim step_id_op_cases; hypsubst_thin?)
   proof -
-    have "\<exists>op2'. step (Inp (Inl p) x) (map_op Inl Inl op) op2' \<and> bisim_cong (\<lambda>op1xx op2xx. \<exists>op. op1xx = comp_op (\<lambda>_. None::0 option) (\<lambda>_. []) op \<I> \<and> op2xx = map_op Inl Inl op) (comp_op (\<lambda>_. None) (\<lambda>_. []) op1' \<I>) op2'"
+    have "\<exists>op2'. step (Inp (Inl p) x) (map_op Inl Inl op) op2' \<and> bisim_R (\<lambda>op1xx op2xx. \<exists>op. op1xx = comp_op (\<lambda>_. None::0 option) (\<lambda>_. []) op \<I> \<and> op2xx = map_op Inl Inl op) (comp_op (\<lambda>_. None) (\<lambda>_. []) op1' \<I>) op2'"
       if "step (Inp p x) op op1'"
       for p :: 'a
         and x :: 'd
         and op1' :: "('a, 'b, 'd) op"
       using that 
       apply -
-      apply (intro conjI[rotated] bc_base exI)
+      apply (intro conjI[rotated] bcr_base exI)
         apply force+
       done
-    moreover have "\<exists>op2'. step (Out (Inl p) x) (map_op Inl Inl op) op2' \<and> bisim_cong (\<lambda>op1xx op2xx. \<exists>op. op1xx = comp_op (\<lambda>_. None::0 option) (\<lambda>_. []) op \<I> \<and> op2xx = map_op Inl Inl op) (comp_op (\<lambda>_. None) (\<lambda>_. []) op1' \<I>) op2'"
+    moreover have "\<exists>op2'. step (Out (Inl p) x) (map_op Inl Inl op) op2' \<and> bisim_R (\<lambda>op1xx op2xx. \<exists>op. op1xx = comp_op (\<lambda>_. None::0 option) (\<lambda>_. []) op \<I> \<and> op2xx = map_op Inl Inl op) (comp_op (\<lambda>_. None) (\<lambda>_. []) op1' \<I>) op2'"
       if "step (Out p x) op op1'"
       for p :: 'b
         and x :: 'd
         and op1' :: "('a, 'b, 'd) op"
       using that 
       apply -
-      apply (intro conjI[rotated] bc_base exI)
+      apply (intro conjI[rotated] bcr_base exI)
         apply force+
       done
-    moreover have "\<exists>op2'. step Tau (map_op Inl Inl op) op2' \<and> bisim_cong (\<lambda>op1xx op2xx. \<exists>op. op1xx = comp_op (\<lambda>_. None::0 option) (\<lambda>_. []) op \<I> \<and> op2xx = map_op Inl Inl op) (comp_op (\<lambda>_. None) (\<lambda>_. []) op1' \<I>) op2'"
+    moreover have "\<exists>op2'. step Tau (map_op Inl Inl op) op2' \<and> bisim_R (\<lambda>op1xx op2xx. \<exists>op. op1xx = comp_op (\<lambda>_. None::0 option) (\<lambda>_. []) op \<I> \<and> op2xx = map_op Inl Inl op) (comp_op (\<lambda>_. None) (\<lambda>_. []) op1' \<I>) op2'"
       if "step Tau op op1'"
       for op1' :: "('a, 'b, 'd) op"
       using that 
       apply -
-      apply (intro conjI[rotated] bc_base exI)
+      apply (intro conjI[rotated] bcr_base exI)
         apply force+
       done
     ultimately show ?thesis
@@ -53,13 +53,13 @@ next
     apply -
     explore (auto elim!: step_map_op_elim step_comp_op_elim step_id_op_cases; hypsubst_thin?)
   proof -
-    have "\<exists>op2'. step (map_IO Inl Inl id io') (comp_op (\<lambda>_. None::0 option) (\<lambda>_. []) op \<I>) op2' \<and> bisim_cong (\<lambda>op1xx op2xx. \<exists>op. op1xx = comp_op (\<lambda>_. None) (\<lambda>_. []) op \<I> \<and> op2xx = map_op Inl Inl op) op2' (map_op Inl Inl op'')"
+    have "\<exists>op2'. step (map_IO Inl Inl id io') (comp_op (\<lambda>_. None::0 option) (\<lambda>_. []) op \<I>) op2' \<and> bisim_R (\<lambda>op1xx op2xx. \<exists>op. op1xx = comp_op (\<lambda>_. None) (\<lambda>_. []) op \<I> \<and> op2xx = map_op Inl Inl op) op2' (map_op Inl Inl op'')"
       if "step io' op op''"
       for io' :: "('a, 'b, 'd) IO"
         and op'' :: "('a, 'b, 'd) op"
       using that 
       apply -
-      apply (intro conjI[rotated] bc_base exI)
+      apply (intro conjI[rotated] bcr_base exI)
       apply force+
       apply (smt (verit, del_insts) IO.map(1) IO.map(3) IO.simps(16) dom_empty empty_iff id_def step_choicesE step_comp_op_L_Inp step_comp_op_L_Out step_comp_op_L_Tau)
       done
@@ -72,38 +72,38 @@ qed
 lemma B2_2:
   \<open>(\<I> :: (0, 0, 'd) op) \<parallel> op ~ map_op Inr Inr op\<close>
   unfolding pcomp_op_def
-proof (coinduction arbitrary: op rule: bisim_coinduct_upto'')
+proof (coinduction arbitrary: op rule: bisim_coinduct)
   case SIM1
   then show ?case 
     apply -
     explore (auto elim!: step_comp_op_elim step_id_op_cases; hypsubst_thin?)
   proof -
-    have "\<exists>op2'a. step (Out (Inr p::0 + 'b) x) (map_op Inr Inr op) op2'a \<and> bisim_cong (\<lambda>op1xx op2xx. \<exists>op. op1xx = comp_op (\<lambda>_. None) (\<lambda>_. []) \<I> op \<and> op2xx = map_op Inr Inr op) (comp_op (\<lambda>_. None) (\<lambda>_. []) \<I> op2') op2'a"
+    have "\<exists>op2'a. step (Out (Inr p::0 + 'b) x) (map_op Inr Inr op) op2'a \<and> bisim_R (\<lambda>op1xx op2xx. \<exists>op. op1xx = comp_op (\<lambda>_. None) (\<lambda>_. []) \<I> op \<and> op2xx = map_op Inr Inr op) (comp_op (\<lambda>_. None) (\<lambda>_. []) \<I> op2') op2'a"
       if "step (Out p x) op op2'"
       for p :: 'b
         and x :: 'd
         and op2' :: "('a, 'b, 'd) op"
      using that 
       apply -
-      apply (intro conjI[rotated] bc_base exI)
+      apply (intro conjI[rotated] bcr_base exI)
         apply force+
      done
-    moreover have "\<exists>op2'a. step (Inp (Inr p::0 + 'a) x) (map_op Inr Inr op) op2'a \<and> bisim_cong (\<lambda>op1xx op2xx. \<exists>op. op1xx = comp_op (\<lambda>_. None) (\<lambda>_. []) \<I> op \<and> op2xx = map_op Inr Inr op) (comp_op (\<lambda>_. None) (\<lambda>_. []) \<I> op2') op2'a"
+    moreover have "\<exists>op2'a. step (Inp (Inr p::0 + 'a) x) (map_op Inr Inr op) op2'a \<and> bisim_R (\<lambda>op1xx op2xx. \<exists>op. op1xx = comp_op (\<lambda>_. None) (\<lambda>_. []) \<I> op \<and> op2xx = map_op Inr Inr op) (comp_op (\<lambda>_. None) (\<lambda>_. []) \<I> op2') op2'a"
       if "step (Inp p x) op op2'"
       for p :: 'a
         and x :: 'd
         and op2' :: "('a, 'b, 'd) op"
      using that 
       apply -
-      apply (intro conjI[rotated] bc_base exI)
+      apply (intro conjI[rotated] bcr_base exI)
         apply force+
      done
-   moreover have "\<exists>op2'a. step Tau (map_op Inr Inr op) op2'a \<and> bisim_cong (\<lambda>op1xx op2xx. \<exists>op. op1xx = comp_op (\<lambda>_. None) (\<lambda>_. []) (\<I>::(0, _, 'd) op) op \<and> op2xx = map_op Inr Inr op) (comp_op (\<lambda>_. None) (\<lambda>_. []) \<I> op2') op2'a"
+   moreover have "\<exists>op2'a. step Tau (map_op Inr Inr op) op2'a \<and> bisim_R (\<lambda>op1xx op2xx. \<exists>op. op1xx = comp_op (\<lambda>_. None) (\<lambda>_. []) (\<I>::(0, _, 'd) op) op \<and> op2xx = map_op Inr Inr op) (comp_op (\<lambda>_. None) (\<lambda>_. []) \<I> op2') op2'a"
       if "step Tau op op2'"
       for op2' :: "('a, 'b, 'd) op"
      using that 
       apply -
-      apply (intro conjI[rotated] bc_base exI)
+      apply (intro conjI[rotated] bcr_base exI)
         apply force+
      done
    ultimately show ?thesis
@@ -115,13 +115,13 @@ next
     apply -
     explore (auto elim!: step_map_op_elim step_comp_op_elim step_id_op_cases; hypsubst_thin?)
   proof -
-    have "\<exists>op2'. step (map_IO Inr Inr id io') (comp_op (\<lambda>_. None) (\<lambda>_. []) (\<I>::(0, _, 'd) op) op) op2' \<and> bisim_cong (\<lambda>op1xx op2xx. \<exists>op. op1xx = comp_op (\<lambda>_. None) (\<lambda>_. []) \<I> op \<and> op2xx = map_op Inr Inr op) op2' (map_op Inr Inr op'')"
+    have "\<exists>op2'. step (map_IO Inr Inr id io') (comp_op (\<lambda>_. None) (\<lambda>_. []) (\<I>::(0, _, 'd) op) op) op2' \<and> bisim_R (\<lambda>op1xx op2xx. \<exists>op. op1xx = comp_op (\<lambda>_. None) (\<lambda>_. []) \<I> op \<and> op2xx = map_op Inr Inr op) op2' (map_op Inr Inr op'')"
       if "step io' op op''"
       for io' :: "('a, 'b, 'd) IO"
         and op'' :: "('a, 'b, 'd) op"
       using that 
       apply -
-      apply (intro conjI[rotated] bc_base exI)
+      apply (intro conjI[rotated] bcr_base exI)
       apply force+
       apply (cases io'; simp)
       subgoal
