nondeterministic_dataflow/table_2/A3.thy
@@ -17,8 +17,6 @@ lemma A3_gen:
   using assms proof (coinduction arbitrary: buf1 buf2 buf3 rule: wbisim_coinduct_upto'')
   case SIM1
   then show ?case 
-    apply - 
-    explore (auto elim !: step_map_op_elim step_comp_op_elim step_id_op_cases step_aeq_op_elim split: if_splits; hypsubst_thin?)
   proof -
     have "\<exists>op2'. wstep (Inp (Inr pb::0 + 'a) xb) (map_op projl projr (comp_op (Some::0 \<Rightarrow> _ option) (\<lambda>_. []) ! (map_op projl projr (comp_op Some (\<lambda>_. []) \<oslash> \<I>)))) op2' \<and> wbisim_cong (\<lambda>op1xx op2xx. (\<exists>buf1 buf2 buf3. op1xx = map_op projl projr (comp_op Some (case_sum (\<lambda>_. []) buf2) (comp_op (\<lambda>_. None) (\<lambda>_. []) (map_op projl projr (comp_op Some (\<lambda>_. []) \<oslash> \<I>)) (id_op buf1)) (aeq_op (case_sum (\<lambda>_. []) buf3)))) \<and> op2xx = map_op projl projr (comp_op (Some::0 \<Rightarrow> _ option) (\<lambda>_. []) ! (map_op projl projr (comp_op Some (\<lambda>_. []) \<oslash> \<I>)))) (map_op projl projr (comp_op Some (case_sum (\<lambda>_. []) buf2) (comp_op (\<lambda>_. None) (\<lambda>_. []) (map_op projl projr (comp_op Some (\<lambda>_. []) \<oslash> \<I>)) (id_op (BENQ pb xb buf1))) (aeq_op (case_sum (\<lambda>_. []) buf3)))) op2'"
       if "pb \<notin> defaults"
@@ -53,8 +51,6 @@ lemma A3_gen:
 next
   case SIM2
   then show ?case 
-    apply -
-    explore (auto elim !: step_map_op_elim step_sink_op step_comp_op_elim step_id_op_cases step_aeq_op_elim split: if_splits; hypsubst_thin)
   proof -
     have "\<exists>op2'. wstep (Inp pa xa) (map_op projl projr (comp_op Some (case_sum (\<lambda>_. []) buf2) (comp_op (\<lambda>_. None) (\<lambda>_. []) (map_op projl projr (comp_op Some (\<lambda>_. []) \<oslash> \<I>)) (id_op buf1)) (aeq_op (case_sum (\<lambda>_. []) buf3)))) op2' \<and> wbisim_cong (\<lambda>op1xx op2xx. (\<exists>buf1 buf2 buf3. op1xx = map_op projl projr (comp_op Some (case_sum (\<lambda>_. []) buf2) (comp_op (\<lambda>_. None) (\<lambda>_. []) (map_op projl projr (comp_op Some (\<lambda>_. []) \<oslash> \<I>)) (id_op buf1)) (aeq_op (case_sum (\<lambda>_. []) buf3)))) \<and> op2xx = map_op projl projr (comp_op (Some::0 \<Rightarrow> _ option) (\<lambda>_. []) ! (map_op projl projr (comp_op Some (\<lambda>_. []) \<oslash> \<I>)))) op2' (map_op projl projr (comp_op (Some::0 \<Rightarrow> _ option) (\<lambda>_. []) ! (map_op projl projr (comp_op Some (\<lambda>_. []) \<oslash> \<I>))))"
       if "pa \<notin> defaults"
