nondeterministic_dataflow/table_2/A7.thy
@@ -13,41 +13,41 @@ lemma A7_gen:
     (acopy_op (case_sum buf1 buf1')) (! \<parallel> id_op buf3))
   \<approx> map_op id Inr (id_op (buf1' >> buf2' >> buf3))\<close>
   unfolding pcomp_op_def
-proof (coinduction arbitrary: buf1 buf1' buf2 buf2' buf3 rule: wbisim_coinduct_upto'')
+proof (coinduction arbitrary: buf1 buf1' buf2 buf2' buf3 rule: wbisim_coinduct)
   case SIM1
   then show ?case
   proof -
-    have "\<exists>op2'. wstep (Inp pa xa) (map_op id Inr (id_op ((buf1' >> buf2') >> buf3))) op2' \<and> wbisim_cong (\<lambda>op1 op2. \<exists>buf1 buf1' buf2 buf2' buf3. op1 = map_op projl projr (comp_op Some (case_sum buf2 buf2') (acopy_op (case_sum buf1 buf1')) (comp_op (\<lambda>_. None) (\<lambda>_. []) (sink_op::('a, 'b, 'c) op) (id_op buf3))) \<and> op2 = map_op id Inr (id_op ((buf1' >> buf2') >> buf3))) (map_op projl projr (comp_op Some (case_sum buf2 buf2') (acopy_op (case_sum (BENQ pa xa buf1) (BENQ pa xa buf1'))) (comp_op (\<lambda>_. None) (\<lambda>_. []) sink_op (id_op buf3)))) op2'"
+    have "\<exists>op2'. wstep (Inp pa xa) (map_op id Inr (id_op ((buf1' >> buf2') >> buf3))) op2' \<and> wbisim_R (\<lambda>op1 op2. \<exists>buf1 buf1' buf2 buf2' buf3. op1 = map_op projl projr (comp_op Some (case_sum buf2 buf2') (acopy_op (case_sum buf1 buf1')) (comp_op (\<lambda>_. None) (\<lambda>_. []) (sink_op::('a, 'b, 'c) op) (id_op buf3))) \<and> op2 = map_op id Inr (id_op ((buf1' >> buf2') >> buf3))) (map_op projl projr (comp_op Some (case_sum buf2 buf2') (acopy_op (case_sum (BENQ pa xa buf1) (BENQ pa xa buf1'))) (comp_op (\<lambda>_. None) (\<lambda>_. []) sink_op (id_op buf3)))) op2'"
       if "pa \<notin> defaults"
       for pa :: 'a
         and xa :: 'c
       using that by force
-    moreover have "\<exists>op2'. wstep (Out (Inr pb::'b + 'a) (BHD pb buf3)) (map_op id Inr (id_op ((buf1' >> buf2') >> buf3))) op2' \<and> wbisim_cong (\<lambda>op1 op2. \<exists>buf1 buf1' buf2 buf2' buf3. op1 = map_op projl projr (comp_op Some (case_sum buf2 buf2') (acopy_op (case_sum buf1 buf1')) (comp_op (\<lambda>_. None) (\<lambda>_. []) sink_op (id_op buf3))) \<and> op2 = map_op id Inr (id_op ((buf1' >> buf2') >> buf3))) (map_op projl projr (comp_op Some (case_sum buf2 buf2') (acopy_op (case_sum buf1 buf1')) (comp_op (\<lambda>_. None) (\<lambda>_. []) sink_op (id_op (BTL pb buf3))))) op2'"
+    moreover have "\<exists>op2'. wstep (Out (Inr pb::'b + 'a) (BHD pb buf3)) (map_op id Inr (id_op ((buf1' >> buf2') >> buf3))) op2' \<and> wbisim_R (\<lambda>op1 op2. \<exists>buf1 buf1' buf2 buf2' buf3. op1 = map_op projl projr (comp_op Some (case_sum buf2 buf2') (acopy_op (case_sum buf1 buf1')) (comp_op (\<lambda>_. None) (\<lambda>_. []) sink_op (id_op buf3))) \<and> op2 = map_op id Inr (id_op ((buf1' >> buf2') >> buf3))) (map_op projl projr (comp_op Some (case_sum buf2 buf2') (acopy_op (case_sum buf1 buf1')) (comp_op (\<lambda>_. None) (\<lambda>_. []) sink_op (id_op (BTL pb buf3))))) op2'"
       if "pb \<notin> defaults"
         and "buf3 pb \<noteq> []"
       for pb :: 'a
-      using that by (fastforce del: wbc_base intro!: wbc_base)
-    moreover have "\<exists>op2'. (step Tau)\<^sup>*\<^sup>* (map_op id Inr (id_op ((buf1' >> buf2') >> buf3))) op2' \<and> wbisim_cong (\<lambda>op1 op2. \<exists>buf1 buf1' buf2 buf2' buf3. op1 = map_op projl projr (comp_op Some (case_sum buf2 buf2') (acopy_op (case_sum buf1 buf1')) (comp_op (\<lambda>_. None) (\<lambda>_. []) (sink_op::('a, 'b, 'c) op) (id_op buf3))) \<and> op2 = map_op id Inr (id_op ((buf1' >> buf2') >> buf3))) (map_op projl projr (comp_op Some (case_sum (BENQ pa (BHD pa buf1) buf2) buf2') (acopy_op (case_sum (BTL pa buf1) buf1')) (comp_op (\<lambda>_. None) (\<lambda>_. []) sink_op (id_op buf3)))) op2'"
+      using that by (fastforce del: wbcr_base intro!: wbcr_base)
+    moreover have "\<exists>op2'. (step Tau)\<^sup>*\<^sup>* (map_op id Inr (id_op ((buf1' >> buf2') >> buf3))) op2' \<and> wbisim_R (\<lambda>op1 op2. \<exists>buf1 buf1' buf2 buf2' buf3. op1 = map_op projl projr (comp_op Some (case_sum buf2 buf2') (acopy_op (case_sum buf1 buf1')) (comp_op (\<lambda>_. None) (\<lambda>_. []) (sink_op::('a, 'b, 'c) op) (id_op buf3))) \<and> op2 = map_op id Inr (id_op ((buf1' >> buf2') >> buf3))) (map_op projl projr (comp_op Some (case_sum (BENQ pa (BHD pa buf1) buf2) buf2') (acopy_op (case_sum (BTL pa buf1) buf1')) (comp_op (\<lambda>_. None) (\<lambda>_. []) sink_op (id_op buf3)))) op2'"
       if "buf1 pa \<noteq> []"
         and "pa \<notin> defaults"
       for pa :: 'a
       using that by force
-    moreover have "\<exists>op2'. (step Tau)\<^sup>*\<^sup>* (map_op id Inr (id_op ((buf1' >> buf2') >> buf3))) op2' \<and> wbisim_cong (\<lambda>op1 op2. \<exists>buf1 buf1' buf2 buf2' buf3. op1 = map_op projl projr (comp_op Some (case_sum buf2 buf2') (acopy_op (case_sum buf1 buf1')) (comp_op (\<lambda>_. None) (\<lambda>_. []) (sink_op::('a, 'b, 'c) op) (id_op buf3))) \<and> op2 = map_op id Inr (id_op ((buf1' >> buf2') >> buf3))) (map_op projl projr (comp_op Some (case_sum buf2 (BENQ pa (BHD pa buf1') buf2')) (acopy_op (case_sum buf1 (BTL pa buf1'))) (comp_op (\<lambda>_. None) (\<lambda>_. []) sink_op (id_op buf3)))) op2'"
+    moreover have "\<exists>op2'. (step Tau)\<^sup>*\<^sup>* (map_op id Inr (id_op ((buf1' >> buf2') >> buf3))) op2' \<and> wbisim_R (\<lambda>op1 op2. \<exists>buf1 buf1' buf2 buf2' buf3. op1 = map_op projl projr (comp_op Some (case_sum buf2 buf2') (acopy_op (case_sum buf1 buf1')) (comp_op (\<lambda>_. None) (\<lambda>_. []) (sink_op::('a, 'b, 'c) op) (id_op buf3))) \<and> op2 = map_op id Inr (id_op ((buf1' >> buf2') >> buf3))) (map_op projl projr (comp_op Some (case_sum buf2 (BENQ pa (BHD pa buf1') buf2')) (acopy_op (case_sum buf1 (BTL pa buf1'))) (comp_op (\<lambda>_. None) (\<lambda>_. []) sink_op (id_op buf3)))) op2'"
       if "buf1' pa \<noteq> []"
         and "pa \<notin> defaults"
       for pa :: 'a
       using that by force
-    moreover have "\<exists>op2'. (step Tau)\<^sup>*\<^sup>* (map_op id Inr (id_op ((buf1' >> buf2') >> buf3))) op2' \<and> wbisim_cong (\<lambda>op1 op2. \<exists>buf1 buf1' buf2 buf2' buf3. op1 = map_op projl projr (comp_op Some (case_sum buf2 buf2') (acopy_op (case_sum buf1 buf1')) (comp_op (\<lambda>_. None) (\<lambda>_. []) (sink_op::('a, 'b, 'c) op) (id_op buf3))) \<and> op2 = map_op id Inr (id_op ((buf1' >> buf2') >> buf3))) (map_op projl projr (comp_op Some (case_sum (BTL pb buf2) buf2') (acopy_op (case_sum buf1 buf1')) (comp_op (\<lambda>_. None) (\<lambda>_. []) sink_op (id_op buf3)))) op2'"
+    moreover have "\<exists>op2'. (step Tau)\<^sup>*\<^sup>* (map_op id Inr (id_op ((buf1' >> buf2') >> buf3))) op2' \<and> wbisim_R (\<lambda>op1 op2. \<exists>buf1 buf1' buf2 buf2' buf3. op1 = map_op projl projr (comp_op Some (case_sum buf2 buf2') (acopy_op (case_sum buf1 buf1')) (comp_op (\<lambda>_. None) (\<lambda>_. []) (sink_op::('a, 'b, 'c) op) (id_op buf3))) \<and> op2 = map_op id Inr (id_op ((buf1' >> buf2') >> buf3))) (map_op projl projr (comp_op Some (case_sum (BTL pb buf2) buf2') (acopy_op (case_sum buf1 buf1')) (comp_op (\<lambda>_. None) (\<lambda>_. []) sink_op (id_op buf3)))) op2'"
       if "buf2 pb \<noteq> []"
         and "pb \<notin> defaults"
       for pb :: 'a
       using that by force
-    moreover have "\<exists>op2'. (step Tau)\<^sup>*\<^sup>* (map_op id Inr (id_op ((buf1' >> buf2') >> buf3))) op2' \<and> wbisim_cong (\<lambda>op1 op2. \<exists>buf1 buf1' buf2 buf2' buf3. op1 = map_op projl projr (comp_op Some (case_sum buf2 buf2') (acopy_op (case_sum buf1 buf1')) (comp_op (\<lambda>_. None) (\<lambda>_. []) (sink_op::('a, 'b, 'c) op) (id_op buf3))) \<and> op2 = map_op id Inr (id_op ((buf1' >> buf2') >> buf3))) (map_op projl projr (comp_op Some (case_sum buf2 (BTL pb buf2')) (acopy_op (case_sum buf1 buf1')) (comp_op (\<lambda>_. None) (\<lambda>_. []) sink_op (id_op (BENQ pb (BHD pb buf2') buf3))))) op2'"
+    moreover have "\<exists>op2'. (step Tau)\<^sup>*\<^sup>* (map_op id Inr (id_op ((buf1' >> buf2') >> buf3))) op2' \<and> wbisim_R (\<lambda>op1 op2. \<exists>buf1 buf1' buf2 buf2' buf3. op1 = map_op projl projr (comp_op Some (case_sum buf2 buf2') (acopy_op (case_sum buf1 buf1')) (comp_op (\<lambda>_. None) (\<lambda>_. []) (sink_op::('a, 'b, 'c) op) (id_op buf3))) \<and> op2 = map_op id Inr (id_op ((buf1' >> buf2') >> buf3))) (map_op projl projr (comp_op Some (case_sum buf2 (BTL pb buf2')) (acopy_op (case_sum buf1 buf1')) (comp_op (\<lambda>_. None) (\<lambda>_. []) sink_op (id_op (BENQ pb (BHD pb buf2') buf3))))) op2'"
       if "buf2' pb \<noteq> []"
         and "pb \<notin> defaults"
       for pb :: 'a
       using that
-      by (intro exI conjI[rotated, OF wbc_base], simp, metis BAPPEND_BENQ_BHD BULK_BENQ_assoc rtranclp.rtrancl_refl)
+      by (intro exI conjI[rotated, OF wbcr_base], simp, metis BAPPEND_BENQ_BHD BULK_BENQ_assoc rtranclp.rtrancl_refl)
     ultimately show ?thesis
       using SIM1 by (auto elim !: step_map_op_elim step_comp_op_elim step_acopy_op_elim step_sink_op step_id_op_cases)
   qed
@@ -55,7 +55,7 @@ next
   case SIM2
   then show ?case
     by (elim exE conjE step_map_op_elim step_id_op_cases; simp split: if_splits)
-      (fastforce del: wbc_base intro!: wbc_base)+
+      (fastforce del: wbcr_base intro!: wbcr_base)+
 qed
 
 lemma A7:
