nondeterministic_dataflow/table_2/A8.thy
@@ -9,14 +9,10 @@ section \<open>Axiom A8: Acopy dummy source\<close>
 
 lemma A8:
   \<open>(\<exclamdown> \<bullet> \<C>) ~ \<exclamdown> \<parallel> \<exclamdown>\<close>
-  apply (coinduction rule: bisim_coinduct_upto)
-  unfolding sim_def
-  apply (rule conjI)
+  apply (coinduction rule: bisim_coinduct)
   subgoal
     unfolding scomp_op_def pcomp_op_def
-    apply (subst comp_op_code)
-    apply (subst acopy_op_code)
-    apply auto
+    apply (auto elim!: step_map_op_elim step_comp_op_elim step_acopy_op_elim step_id_op_cases)
     done
   subgoal
     apply (metis cempty_iff choices_pcomp_op_dummy_source step_choicesE)
